translator/lean/corellzk2smt/Corellzk2smt/SymExec/PartialCorrectness/ProgCorrectness.lean
@@ -84,7 +84,7 @@ open Corellzk2smt.FFConstraints.Satisfiability
 open Corellzk2smt.FFConstraints.Satisfiability_th
 open Corellzk2smt.SymExec.Lemmas
 open Corellzk2smt.SymExec.PartialCorrectness.Correctness
-open Corellzk2smt.SymExec.FuncCorrectness
+open Corellzk2smt.SymExec.PartialCorrectness.FuncCorrectness
 open Corellzk2smt.SymExec.PartialCorrectness.FuncCallCorrectness
 open Corellzk2smt.SymExec.ProgCorrectness
 open Corellzk2smt.SymExec.PartialCorrectness.Lemmas
